ott_coq/destination_calculus_proofs.v
@@ -245,7 +245,7 @@ Proof. Admitted.
 Lemma DisjointTohdns_Disjoint : forall (D D' : ctx), ctx_Disjoint D D' -> hdns_Disjoint hnamesᴳ(D) hnamesᴳ(D').
 Proof. Admitted.
 
-Lemma hdns_max_hnames_Disjoint : forall (H H' : hdns) (h' : hdn), ʰmax(H) <= h' -> hdns_Disjoint H (H' ᴴ⩲ h').
+Lemma hdns_max_hdns_Disjoint : forall (H H' : hdns) (h' : hdn), ʰmax(H) <= h' -> hdns_Disjoint H (H' ᴴ⩲ h').
 Proof. Admitted.
 
 Lemma SubsetCtxUnionBackward : forall (G G': ctx) (H: hdns), HdnsM.Subset hnamesᴳ(G ⨄ G') H -> HdnsM.Subset hnamesᴳ(G) H /\ HdnsM.Subset hnamesᴳ(G') H.
@@ -279,7 +279,7 @@ Proof. Admitted.
 Ltac hauto_ctx :=
   hauto
     depth: 3
-    use: ValidOnlyUnionBackward, ValidOnlyUnionForward, ValidOnlyStimesEquiv, ValidOnlyMinusEquiv, ValidOnlyHdnShiftEquiv, DestOnlyUnionEquiv, DestOnlyStimesEquiv, DestOnlyHdnShiftEquiv, LinNuOnlyUnionEquiv, LinNuOnlyStimesEquiv, LinNuOnlyHdnShiftEquiv, LinOnlyUnionEquiv, LinOnlyStimesEquiv, LinOnlyHdnShiftEquiv, LinNuOnlyWkLinOnly, LinOnlyWkValidOnly, IsLinNuWkIsLin, IsLinWkIsValid, DisjointStimesLeftEquiv, DisjointStimesRightEquiv, DisjointMinusLeftEquiv, DisjointMinusRightEquiv, DisjointNestedLeftEquiv, DisjointNestedRightEquiv, DisjointHdnShiftEq, DisjointCommutative, EmptyIsLinOnly, EmptyIsDestOnly, EmptyIsDisjointLeft, EmptyIsDisjointRight, StimesEmptyEq, MinusEmptyEq, UnionIdentityRight, UnionIdentityLeft, DisjointDestOnlyVar, UnionCommutative, UnionAssociative, UnionHdnShiftEq, StimesHdnShiftEq, StimesIsAction, StimesUnionDistributive, StimesIdentity, TimesCommutative, TimesAssociative, TimesIdentityRight, TimesIdentityLeft, hnames_CWkhnames_G, hnames_DisjointToDisjoint, DisjointTohdns_Disjoint, hdns_max_hnames_Disjoint, UnionIdentityRight, UnionIdentityLeft, SubsetCtxUnionBackward, HmaxSubset, hnamesMinusEq, hnamesFullShiftEq, hnamesEmpty, EmptyIshdns_DisjointRight, EmptyIshdns_DisjointLeft, MinusHdnShiftEq, CompatibleDestSingleton, IncompatibleVarDestOnly, MinusSingletonEq, FinAgeOnlyUnionEquiv, FinAgeOnlyStimesEquiv, FinAgeOnlyHdnShiftEquiv, EmptyIsFinAgeOnly.
+    use: ValidOnlyUnionBackward, ValidOnlyUnionForward, ValidOnlyStimesEquiv, ValidOnlyMinusEquiv, ValidOnlyHdnShiftEquiv, DestOnlyUnionEquiv, DestOnlyStimesEquiv, DestOnlyHdnShiftEquiv, LinNuOnlyUnionEquiv, LinNuOnlyStimesEquiv, LinNuOnlyHdnShiftEquiv, LinOnlyUnionEquiv, LinOnlyStimesEquiv, LinOnlyHdnShiftEquiv, LinNuOnlyWkLinOnly, LinOnlyWkValidOnly, IsLinNuWkIsLin, IsLinWkIsValid, DisjointStimesLeftEquiv, DisjointStimesRightEquiv, DisjointMinusLeftEquiv, DisjointMinusRightEquiv, DisjointNestedLeftEquiv, DisjointNestedRightEquiv, DisjointHdnShiftEq, DisjointCommutative, EmptyIsLinOnly, EmptyIsDestOnly, EmptyIsDisjointLeft, EmptyIsDisjointRight, StimesEmptyEq, MinusEmptyEq, UnionIdentityRight, UnionIdentityLeft, DisjointDestOnlyVar, UnionCommutative, UnionAssociative, UnionHdnShiftEq, StimesHdnShiftEq, StimesIsAction, StimesUnionDistributive, StimesIdentity, TimesCommutative, TimesAssociative, TimesIdentityRight, TimesIdentityLeft, hnames_CWkhnames_G, hnames_DisjointToDisjoint, DisjointTohdns_Disjoint, hdns_max_hdns_Disjoint, UnionIdentityRight, UnionIdentityLeft, SubsetCtxUnionBackward, HmaxSubset, hnamesMinusEq, hnamesFullShiftEq, hnamesEmpty, EmptyIshdns_DisjointRight, EmptyIshdns_DisjointLeft, MinusHdnShiftEq, CompatibleDestSingleton, IncompatibleVarDestOnly, MinusSingletonEq, FinAgeOnlyUnionEquiv, FinAgeOnlyStimesEquiv, FinAgeOnlyHdnShiftEquiv, EmptyIsFinAgeOnly.
 
 Ltac crush :=
   solve
@@ -556,7 +556,7 @@ Proof.
               assert (ʰmax(hnamesᴳ(D2)) <= ʰmax(hnamesꟲ(C))).
               { apply HmaxSubset. tauto. }
               assert (hdns_Disjoint hnamesᴳ(D2) (hnamesᴳ(D13) ᴴ⩲ ʰmax( hnamesꟲ( C)))).
-              { apply hdns_max_hnames_Disjoint. tauto. }
+              { apply hdns_max_hdns_Disjoint. tauto. }
               assert (hdns_Disjoint hnamesᴳ(D2)  hnamesᴳ( D13 ᴳ[ hnamesᴳ( ᴳ- D13) ⩲ ʰmax( hnamesꟲ( C))])).
               { rewrite hnamesMinusEq. rewrite hnamesFullShiftEq. tauto. }
               apply hnames_DisjointToDisjoint; crush.
@@ -566,7 +566,7 @@ Proof.
               assert (ʰmax(hnamesᴳ(D11)) <= ʰmax(hnamesꟲ(C))).
               { apply HmaxSubset. tauto. }
               assert (hdns_Disjoint hnamesᴳ(D11) (hnamesᴳ(D13) ᴴ⩲ ʰmax( hnamesꟲ( C)))).
-              { apply hdns_max_hnames_Disjoint. tauto. }
+              { apply hdns_max_hdns_Disjoint. tauto. }
               assert (hdns_Disjoint hnamesᴳ(D11)  hnamesᴳ( D13 ᴳ[ hnamesᴳ( ᴳ- D13) ⩲ ʰmax( hnamesꟲ( C))])).
               { rewrite hnamesMinusEq. rewrite hnamesFullShiftEq. tauto. }
               apply hnames_DisjointToDisjoint; crush.
@@ -602,7 +602,7 @@ Proof.
               assert (ʰmax(hnamesᴳ(D2)) <= ʰmax(hnamesꟲ(C))).
               { apply HmaxSubset. tauto. }
               assert (hdns_Disjoint hnamesᴳ(D2) (hnamesᴳ(D13) ᴴ⩲ ʰmax( hnamesꟲ( C)))).
-              { apply hdns_max_hnames_Disjoint. tauto. }
+              { apply hdns_max_hdns_Disjoint. tauto. }
               assert (hdns_Disjoint hnamesᴳ(D2)  hnamesᴳ( D13 ᴳ[ hnamesᴳ( ᴳ- D13) ⩲ ʰmax( hnamesꟲ( C))])).
               { rewrite hnamesMinusEq. rewrite hnamesFullShiftEq. tauto. }
               apply hnames_DisjointToDisjoint; crush.
@@ -612,14 +612,14 @@ Proof.
               assert (ʰmax(hnamesᴳ(D11)) <= ʰmax(hnamesꟲ(C))).
               { apply HmaxSubset. tauto. }
               assert (hdns_Disjoint hnamesᴳ(D11) (hnamesᴳ(D13) ᴴ⩲ ʰmax( hnamesꟲ( C)))).
-              { apply hdns_max_hnames_Disjoint. tauto. }
+              { apply hdns_max_hdns_Disjoint. tauto. }
               assert (hdns_Disjoint hnamesᴳ(D11)  hnamesᴳ( D13 ᴳ[ hnamesᴳ( ᴳ- D13) ⩲ ʰmax( hnamesꟲ( C))])).
               { rewrite hnamesMinusEq. rewrite hnamesFullShiftEq. tauto. }
               apply hnames_DisjointToDisjoint; crush.
             }
           } } { crush. } { crush. } { crush. } { crush. } { crush. } { crush. } { rewrite UnionCommutative in TyC. rewrite UnionAssociative in TyC. tauto. }
           { rewrite <- D12Eq. rewrite <- MinusHdnShiftEq. rewrite <- UnionHdnShiftEq. apply TyR_v_hdn_shift. tauto.  }
-          { rewrite <- MinusHdnShiftEq. rewrite hnamesFullShiftEq. apply hdns_max_hnames_Disjoint with (h' := ʰmax( hnamesꟲ( C))). reflexivity. }
+          { rewrite <- MinusHdnShiftEq. rewrite hnamesFullShiftEq. apply hdns_max_hdns_Disjoint with (h' := ʰmax( hnamesꟲ( C))). reflexivity. }
     - (* Sem-eterm-AOpenUnfoc *)
       inversion Tyt; subst. rename TyC into TyCc, TyRv into TyRv1. clear H2.
       inversion TyCc; subst. rename H6 into hdnsDisjoint.
